

* 12.1

$$\begin{cases} -u''(x) = f(x) & 0 < x < 1 \\ u(0) = u(1) = 0 \end{cases}$$

by 12.3) $u(x) = \int_0^x G(x,s)f(s)ds + \int_x^1 x(1-s)f(s)ds$

$$G(x,s) = \begin{cases} s(1-x) & 0 \leq s \leq x \\ x(1-s) & x \leq s \leq 1 \end{cases}$$

for $f(s) = \frac{1}{s}$ $u(x) = \int_0^x s(1-x) \frac{1}{s} ds + \int_x^1 x(1-s) \frac{1}{s} ds$
 $= (1-x) \int_0^x 1 ds + x \int_x^1 (\frac{1}{s} - 1) ds$
 $= (1-x)(x-0) + x(\ln s - s) \Big|_x^1$
 $= x - x^2 + x(-1 - \ln x + x) = -x \ln x$

when $0 < x < 1 \Rightarrow u = -x \ln x \in C^2(0,1)$

$$u(x) = -x \ln x$$

$$u'(x) = -\ln x - 1$$

$$u''(x) = -\frac{1}{x}$$

$\ln 0, \frac{1}{0}$ not exist $\Rightarrow u(0), u'(0), u''(0)$ not exist

$$\begin{aligned} 2. \sum_{j=0}^{n-1} (w_{j+1} - w_j) v_j &= \sum_{j=0}^{n-1} w_{j+1} v_j - \sum_{j=0}^{n-1} w_j v_j \\ &= \sum_{j=1}^n w_j v_{j-1} - \sum_{j=0}^{n-1} w_j v_j \\ &= w_n v_{n-1} - w_0 v_0 + \sum_{j=1}^{n-1} w_j (v_{j-1} - v_j) + w_n v_n - w_n v_n \\ &= w_n v_n - w_0 v_0 + \sum_{j=1}^{n-1} w_j (v_{j-1} - v_j) - (v_n - v_{n-1}) w_n \\ &= w_n v_n - w_0 v_0 - \sum_{j=0}^{n-1} (v_{j+1} - v_j) w_{j+1} \end{aligned}$$

for $V_n^0 = \{v_n : v_0 = 0, v_n = 0\}$

$$(L_h v)_j = -\frac{v_{j+1} - 2v_j + v_{j-1}}{h^2}$$

$$(u, v)_h = h \sum_{j=1}^{n-1} u_j v_j$$

$$\begin{aligned} \Rightarrow (L_h v_n, v_n)_h &= h \sum_{j=1}^{n-1} (L_h v)_j v_j = -\frac{h}{h^2} \sum_{j=1}^{n-1} (v_{j+1} - 2v_j + v_{j-1}) v_j \quad \text{let } w_j = v_j - v_{j-1} \\ &= -\frac{1}{h} \sum_{j=1}^{n-1} (w_{j+1} - w_j) v_j \quad \because v_0 = 0 \\ &= -\frac{1}{h} \sum_{j=0}^{n-1} (w_{j+1} - w_j) v_j \quad \text{by above} \\ &= -\frac{1}{h} (w_n v_n - w_0 v_0 - \sum_{j=0}^{n-1} (v_{j+1} - v_j) w_{j+1}) \\ &= -\frac{1}{h} \left[-\sum_{j=0}^{n-1} (v_{j+1} - v_j)^2 \right] = \frac{1}{h} \sum_{j=0}^{n-1} (v_{j+1} - v_j)^2 \end{aligned}$$

*12-6

know that $G(x, s) = \begin{cases} s(1-x) & 0 \leq s \leq x \\ x(1-s) & x \leq s \leq 1 \end{cases}, (L_h V)_j = -\frac{V_{j+1} - 2V_j + V_{j-1}}{h^2}$

$$G^k \in V_n^0$$

$$L_h G^k = e^k, G_0^k = G_{n+1}^k = 0$$

$$\text{let } \tilde{G}_j = h G(x_j, x_k) \quad j = 0, \dots, n+1$$

$$\therefore G(0, x_k) = G(1, x_k) = 0$$

$$\therefore \tilde{G}_0 = h G(0, x_k) = 0, \quad \tilde{G}_{n+1} = h G(1, x_k) = 0$$

$$\therefore G(x, x_k) = \begin{cases} x(1-x_k) & 0 \leq x \leq x_k \\ x_k(1-x) & x_k \leq x \leq 1 \end{cases} \quad \text{when } x_j = jh$$

$$j \leq k \Rightarrow G(x_j, x_k) = x_j(1-x_k) = jh(1-kh) \quad \text{linear}$$

$$j \geq k \Rightarrow G(x_j, x_k) = x_k(1-x_j) = kh(1-jh) \quad \text{linear}$$

$$\text{now for } j \neq k \quad \text{for } a+bj \quad (a+b(j+1)) - 2(a+bj) + (a+b(j-1)) = 0$$

$$\Rightarrow \tilde{G}_{j+1} - 2\tilde{G}_j + \tilde{G}_{j-1} = 0$$

$$\Rightarrow (L_h \tilde{G})_j = -\frac{\tilde{G}_{j+1} - 2\tilde{G}_j + \tilde{G}_{j-1}}{h^2} = 0 \quad (j \neq k)$$

$$\begin{aligned} \text{for } j=k & \Rightarrow (L_h H)_k = -\frac{H_{j+1} - 2H_j + H_{j-1}}{h^2} \\ &= -\frac{1}{h^2} \left(x_k(1-x_{k+1}) - 2x_k(1-x_k) + x_{k-1}(1-x_k) \right) \\ &= -\frac{1}{h^2} (x_k - x_k^2 - x_k h - 2x_k + 2x_k^2 + x_{k-1} - x_k^2 - h + h x_k) \\ &= \frac{1}{h} \end{aligned}$$

$$\Rightarrow (L_h \tilde{G})_k = h(L_h H)_k = h \cdot \frac{1}{h} = 1$$

$$\Rightarrow (L_h \tilde{G})_n = \begin{cases} 1 & j=k \\ 0 & j \neq k \end{cases}, \quad \tilde{G}_0 = \tilde{G}_{n+1} = 0$$

$$\therefore G^k(x_j) = \tilde{G}_j = h G(x_j, x_k)$$